SeqNatToNat.dfy
@@ -600,10 +600,45 @@ module SeqNatToNat {
     NatsToNat(bound_ns)
   }
 
-  lemma {:vcs_split_on_every_assert} NatsToNatBounded(a: seq<nat>, bound: nat)
-    requires |a| > 0
-    requires forall i : nat :: i < |a| ==> a[i] < bound
-    ensures NatsToNat(a) < NatsToNatBound(|a|, bound)
+  function {:vcs_split_on_every_assert} ArbLenNatsToNatBound(max_length: nat, bound: nat): nat
+    requires max_length > 0
   {
+    var bound_ns := seq(max_length, i requires 0 <= i < max_length => bound);
+    ArbLenNatsToNat(bound_ns)
+  }
+
+  lemma {:vcs_split_on_every_assert} BoundIncreasesWithLength(la: nat, lb: nat, bound: nat)
+    requires la > 0
+    requires lb > la
+    ensures NatsToNatBound(la, bound) < NatsToNatBound(lb, bound)
+  {
+  }
+
+  lemma {:vcs_split_on_every_assert} ArbLenBoundIncreasesWithLength(la: nat, lb: nat, bound: nat)
+    requires la > 0
+    requires lb > la
+    ensures ArbLenNatsToNatBound(la, bound) < ArbLenNatsToNatBound(lb, bound)
+  {
+  }
+
+  lemma {:vcs_split_on_every_assert} ArbLenNatsToNatBounded(a: seq<nat>, max_length: nat, bound: nat)
+    requires |a| > 0
+    requires |a| <= max_length
+    requires forall i : nat :: i < |a| ==> a[i] < bound
+    ensures ArbLenNatsToNat(a) < ArbLenNatsToNatBound(max_length, bound)
+  {
+  }
+
+  lemma ArbLenNatsToNatOutOfBoundElementOutOfBound(a: seq<nat>, max_length: nat, bound: nat)
+    requires |a| > 0
+    requires |a| <= max_length
+    requires ArbLenNatsToNat(a) >= ArbLenNatsToNatBound(max_length, bound)
+    ensures exists i: nat :: i < |a| && a[i] >= bound
+  {
+    if !exists i: nat :: i < |a| && a[i] >= bound {
+      assert forall i: nat :: i< |a| ==> a[i] < bound;
+      ArbLenNatsToNatBounded(a, max_length, bound);
+    } else {
+    }
   }
 }
