CircuitBounds.dfy
@@ -1,0 +1,272 @@
+// Working to prove that HPNP are bounded.
+module CircuitBounds {
+
+    import opened Std.Wrappers
+    import opened Circuit
+    import Seq=Std.Collections.Seq
+
+    function GetSubCRef(lib: CLib, c: Circuit, n: CNode): (r: Option<CircuitRef>)
+        requires CircuitValid(lib, c)
+        ensures r.None? || (CRefCircuitValid(lib, r.value) && CRefHierLevelReduced(lib, c, r.value))
+        ensures c.NodeKind(n).Some? && c.NodeKind(n).value.CHier? ==>
+            r.Some? && (r.value == c.NodeKind(n).value.CRef)
+    {
+        assert CircuitNodeKindValid(lib, c);
+        match c.NodeKind(n)
+            case Some(nk) => (
+                match nk
+                case CHier(cref) =>
+                    assert CNodeKindValid(lib, c, nk);
+                    assert CRefValid(lib, cref);
+                    Some(cref)
+                case _ => None
+            )
+            case _ => None
+    }
+
+    predicate CRefHierLevelReduced(lib: CLib, c: Circuit, cref: CircuitRef)
+        requires CircuitValid(lib, c)
+        requires CRefCircuitValid(lib, cref)
+    {
+        var unref_c := lib.Circuits[cref];
+        unref_c.HierLevel < c.HierLevel
+    }
+
+    function DirectSubCRefsInternal(lib: CLib, c: Circuit, n: CNode, subcircuits: seq<CircuitRef>): (r: seq<CircuitRef>)
+        requires CircuitValid(lib, c)
+        requires forall i: nat :: i < |subcircuits| ==>
+            CRefCircuitValid(lib, subcircuits[i]) && CRefHierLevelReduced(lib, c, subcircuits[i])
+        requires forall m: CNode :: m >= n && c.NodeKind(m).Some? && c.NodeKind(m).value.CHier? ==> c.NodeKind(m).value.CRef in subcircuits
+        ensures forall i: nat :: i < |r| ==> CRefCircuitValid(lib, r[i]) &&
+            CRefHierLevelReduced(lib, c, r[i])
+        ensures forall m: CNode :: c.NodeKind(m).Some? && c.NodeKind(m).value.CHier? ==>
+            c.NodeKind(m).value.CRef in r
+    {
+        if n == 0 then
+            subcircuits
+        else
+            var new_cref := GetSubCRef(lib, c, n-1);
+            var updated_subcircuits: seq<CircuitRef> :=
+                match new_cref
+                    case Some(cref) => subcircuits + [cref]
+                    case None => subcircuits;
+            DirectSubCRefsInternal(lib, c, n-1, updated_subcircuits)
+    }
+
+    function DirectSubCRefs(lib: CLib, c: Circuit): (r: seq<CircuitRef>)
+        requires CircuitValid(lib, c)
+        ensures forall m: CNode :: c.NodeKind(m).Some? && c.NodeKind(m).value.CHier? ==>
+            c.NodeKind(m).value.CRef in r
+        ensures forall cref: CircuitRef :: cref in r ==>
+            CRefCircuitValid(lib, cref) && CRefHierLevelReduced(lib, c, cref)
+    {
+        assert CircuitNodeKindValid(lib, c);
+        assert forall n: CNode :: n >= c.NodeBound ==> c.NodeKind(n).None?;
+        DirectSubCRefsInternal(lib, c, c.NodeBound, [])
+    }
+
+    lemma {:vcs_split_on_every_assert} HierBoundEncloses(
+            lib: CLib, c: Circuit, bound_f: Circuit -> nat, hp: HierarchyPath)
+        requires CircuitValid(lib, c)
+        requires HierarchyPathValid(lib, c, hp)
+        ensures
+            var hierc := HierarchyPathCircuit(lib, c, hp);
+            CircuitValid(lib, hierc) &&
+            HierBound(lib, hierc, bound_f) <= HierBound(lib, c, bound_f)
+        decreases |hp.v|
+    {
+        var hierc := HierarchyPathCircuit(lib, c, hp);
+        HierarchyPathCircuitValid(lib, c, hp);
+        if |hp.v| == 0 {
+            assert HierBound(lib, hierc, bound_f) <= HierBound(lib, c, bound_f);
+        } else {
+            var (head, tail) := HPHeadTail(hp);
+            HierBoundEncloses(lib, c, bound_f, tail);
+            var tail_c := HierarchyPathCircuit(lib, c, tail);
+            HierarchyPathCircuitValid(lib, c, tail);
+            assert HierBound(lib, tail_c, bound_f) <= HierBound(lib, c, bound_f);
+            assert HierBound(lib, hierc, bound_f) <= HierBound(lib, c, bound_f);
+        }
+    }
+
+    function GetSubBounds(lib: CLib, c: Circuit, bound_f: Circuit -> nat): (r: seq<nat>)
+        requires CircuitValid(lib, c)
+        ensures forall m: CNode :: c.NodeKind(m).Some? && c.NodeKind(m).value.CHier? ==>
+            CRefValid(lib, c.NodeKind(m).value.CRef) &&
+            var subc := lib.Circuits[c.NodeKind(m).value.CRef];
+            CircuitValid(lib, subc) &&
+            subc.HierLevel < c.HierLevel &&
+            HierBound(lib, subc, bound_f) in r
+        decreases c.HierLevel, 0
+    {
+        var subcrefs := DirectSubCRefs(lib, c);
+        var new_bound := bound_f(c);
+        assert forall m: CNode :: c.NodeKind(m).Some? && c.NodeKind(m).value.CHier? ==>
+            var subcref := c.NodeKind(m).value.CRef;
+            subcref in subcrefs;
+        var bounds := Seq.Map(
+            cref requires CRefCircuitValid(lib, cref) && CRefHierLevelReduced(lib, c, cref)  =>
+                HierBound(lib, lib.Circuits[cref], bound_f),
+            subcrefs);
+        assert forall m: CNode :: c.NodeKind(m).Some? && c.NodeKind(m).value.CHier? ==>
+            var subcref := c.NodeKind(m).value.CRef;
+            var subc := lib.Circuits[subcref];
+            var index: nat :| index < |subcrefs| && subcrefs[index] == subcref;
+            (bounds[index] == HierBound(lib, subc, bound_f)) &&
+            (HierBound(lib, subc, bound_f) in bounds);
+        bounds
+    }
+
+    function {:vcs_split_on_every_assert} HierBound(lib: CLib, c: Circuit, bound_f: Circuit -> nat): (r: nat)
+        requires CircuitValid(lib, c)
+        ensures forall m: CNode :: c.NodeKind(m).Some? && c.NodeKind(m).value.CHier? ==>
+            CRefValid(lib, c.NodeKind(m).value.CRef) &&
+            var subc := lib.Circuits[c.NodeKind(m).value.CRef];
+            CircuitValid(lib, subc) &&
+            subc.HierLevel < c.HierLevel &&
+            HierBound(lib, subc, bound_f) <= r
+        ensures bound_f(c) as nat <= r
+        decreases c.HierLevel, 1
+    {
+        var bounds := GetSubBounds(lib, c, bound_f);
+        var new_bound := bound_f(c);
+        var combined_bounds := bounds + [new_bound];
+        var max_bound := Seq.Max(combined_bounds);
+        assert new_bound in combined_bounds;
+        assert new_bound <= max_bound;
+        var subcrefs := DirectSubCRefs(lib, c);
+        assert forall pb: nat :: pb in bounds+[new_bound] ==> pb <= max_bound;
+        assert forall m: CNode :: c.NodeKind(m).Some? && c.NodeKind(m).value.CHier? ==>
+            var subcref := c.NodeKind(m).value.CRef;
+            (subcref in subcrefs) && 
+            var subc := lib.Circuits[subcref];
+            (HierBound(lib, subc, bound_f) in bounds + [bound_f(c)]);
+        assert forall m: CNode :: c.NodeKind(m).Some? && c.NodeKind(m).value.CHier? ==>
+            var subcref := c.NodeKind(m).value.CRef;
+            var subc := lib.Circuits[subcref];
+            (HierBound(lib, subc, bound_f) <= max_bound);
+        max_bound
+    }
+
+    // Get a port bound
+    // Show that port bound is bigger or equal to all circuit Port Bounds.
+
+    // Port bound is determined recursively from the top Circuit.
+
+    // Then we get a Subcircuit specified by a HP.
+    // Prove that that it satisfies it by building the HP up from the start.
+
+    function getpb(c: Circuit): nat
+    {
+        c.PortBound as nat
+    }
+
+    function getnb(c: Circuit): nat
+    {
+        c.NodeBound as nat
+    }
+
+    function HierPortBound(lib: CLib, c: Circuit): nat
+        requires CircuitValid(lib, c)
+    {
+        HierBound(lib, c, getpb)
+    }
+
+    function HierNodeBound(lib: CLib, c: Circuit): nat
+        requires CircuitValid(lib, c)
+    {
+        HierBound(lib, c, getnb)
+    }
+
+    lemma SubcircuitInHierPortBound(lib: CLib, c: Circuit, hp: HierarchyPath)
+        requires CircuitValid(lib, c)
+        requires HierarchyPathValid(lib, c, hp)
+        ensures
+            var hier_c := HierarchyPathCircuit(lib, c, hp);
+            hier_c.PortBound as nat <= HierPortBound(lib, c)
+    {
+        HierBoundEncloses(lib, c, getpb, hp);
+    }
+
+
+    lemma SubcircuitInHierNodeBound(lib: CLib, c: Circuit, hp: HierarchyPath)
+        requires CircuitValid(lib, c)
+        requires HierarchyPathValid(lib, c, hp)
+        ensures
+            var hier_c := HierarchyPathCircuit(lib, c, hp);
+            hier_c.NodeBound as nat <= HierNodeBound(lib, c)
+    {
+        HierBoundEncloses(lib, c, getnb, hp);
+    }
+
+    lemma HPInHierNodeBound(lib: CLib, c: Circuit, hp: HierarchyPath)
+        requires CircuitValid(lib, c)
+        requires HierarchyPathValid(lib, c, hp)
+        ensures
+            forall n: CNode :: (n in hp.v) ==> n as nat < HierNodeBound(lib, c)
+        decreases |hp.v|
+    {
+        if |hp.v| == 0 {
+        } else {
+            var (head, tail) := HPHeadTail(hp);
+            var hier_c := HierarchyPathCircuit(lib, c, hp);
+            var tail_c := HierarchyPathCircuit(lib, c, tail);
+            HierarchyPathCircuitValid(lib, c, tail);
+            assert head <= tail_c.NodeBound;
+            SubcircuitInHierNodeBound(lib, c, tail);
+            assert tail_c.NodeBound as nat <= HierNodeBound(lib, c);
+            HPInHierNodeBound(lib, c, tail);
+            assert head as nat <= HierNodeBound(lib, c);
+            assert forall n: CNode :: (n in tail.v) ==> n as nat < HierNodeBound(lib, c);
+            assert forall n: CNode :: (n in tail.v + [head]) ==> n as nat < HierNodeBound(lib, c);
+            assert tail.v + [head] == hp.v;
+        }
+    }
+
+    // Show that the any valid hpnp is smaller than total bound
+
+    ghost function HPNPElementBound(lib: CLib, c: Circuit): nat
+        requires CircuitValid(lib, c)
+    {
+        var max_node_index := HierNodeBound(lib, c);
+        var max_port_index := HierPortBound(lib, c);
+        var max_index := if max_node_index > max_port_index then max_node_index else max_port_index;
+        max_index
+    }
+
+    lemma HPNPElementsInBound(lib: CLib, c: Circuit, hpnp: HPNP)
+        requires CircuitValid(lib, c)
+        requires HPNPValid(lib, c, hpnp)
+        ensures
+            forall n: CNode :: (n in hpnp.hpn.hp.v) ==> n as nat < HPNPElementBound(lib, c)
+        ensures hpnp.hpn.n as nat < HPNPElementBound(lib, c)
+        ensures hpnp.p as nat < HPNPElementBound(lib, c)
+    {
+        var element_bound := HPNPElementBound(lib, c);
+        HPInHierNodeBound(lib, c, hpnp.hpn.hp);
+        var hier_c := HierarchyPathCircuit(lib, c, hpnp.hpn.hp);
+        HierarchyPathCircuitValid(lib, c, hpnp.hpn.hp);
+        SubcircuitInHierNodeBound(lib, c, hpnp.hpn.hp);
+        assert hier_c.NodeBound as nat <= element_bound;
+        SubcircuitInHierPortBound(lib, c, hpnp.hpn.hp);
+        assert hier_c.PortBound as nat <= element_bound;
+        assert CircuitNodeKindValid(lib, hier_c);
+        assert hpnp.p < hier_c.PortBound;
+        assert hpnp.hpn.n < hier_c.NodeBound;
+    }
+
+    ghost function HPNPBound(lib: CLib, c: Circuit): nat
+        requires CircuitValid(lib, c)
+    {
+        var max_index := HPNPElementBound(lib, c);
+        var ns := seq(c.HierLevel+2, i requires 0 <= i < c.HierLevel+2 => max_index);
+        SeqNatToNat.ArbLenNatsToNat(ns)
+    }
+
+    lemma HPNPInBound(lib: CLib, c: Circuit, hpnp: HPNP)
+        requires CircuitValid(lib, c)
+        requires HPNPValid(lib, c, hpnp)
+    {
+    }
+
+}
